\documentclass[12pt]{article}
\usepackage[left=3cm,right=3cm,top=3cm,bottom=3cm]{geometry}
\usepackage{amsmath}
\usepackage{amsthm}
\usepackage{amssymb}
\usepackage{bm}
\usepackage{tabularx}

\begin{document}
\title{Summary of Continuous Distributions for a random Variable $X$}
\author{Dinesh Kalamegam}
\date{\today}
\maketitle

\section{Uniform $X \sim U(a,b)$}
\subsection{Probability Density Function $f(x)$}

\begin{equation*}
  f(x) =
  \begin{cases}
     \frac{1}{b-a} & a \leq x \leq b \\
     0 & \text{Otherwise}
  \end{cases}
\end{equation*}

\subsection{Cumulative Distribution Function $F(x)$}

\begin{equation*}
  F(x) =
  \begin{cases}
     0 & x <a \\
     \frac{x-a}{b-a} & a \leq x \leq b \\
     1 & x>b
  \end{cases}
\end{equation*}

\subsection{Moment Generating Function $M(t)=E(e^{tX})$}

\begin{equation*}
    M(t)=\frac{e^{tb}-e^{ta}}{t(b-a)}
\end{equation*}

\subsection{$\bm{E(X)}$}

\begin{equation*}
  E(X) = \frac{a+b}{2}
\end{equation*}

\subsection{$\bm{Var(X)}$}

\begin{equation*}
  Var(X)= \frac{(b-a)^{2}}{12}
\end{equation*}

\newpage
\section{Exponential $X \sim Exp(\lambda)$}
\subsection{Probability Density Function $f(x)$}

\begin{equation*}
  f(x) =
  \begin{cases}
     \lambda e^{-\lambda x} & x>0 \\
     0 & \text{Otherwise}
  \end{cases}
\end{equation*}

\subsection{Cumulative Distribution Function $F(x)$}
\begin{align*}
  F(x) &= 1-e^{-\lambda x} \text{ where $x>0$}\\
\end{align*}

\subsection{Moment Generating Function $M(t)=E(e^{tX})$}

\begin{equation*}
    M(t)=\frac{\lambda}{\lambda -t}
\end{equation*}

\subsection{$\bm{E(X)}$}

\begin{equation*}
  E(X) = \frac{1}{\lambda}
\end{equation*}

\subsection{$\bm{Var(X)}$}

\begin{equation*}
  Var(X)= \frac{1}{\lambda^{2}}
\end{equation*}

\newpage
\section{Gamma $X \sim \Gamma(\alpha,\lambda)$}
\subsection{Probability Density Function $f(x)$}

\begin{equation*}
  f(x) =
  \begin{cases}
     \frac{\lambda^{\alpha} x^{\alpha -1} e^{-\lambda x}}{\Gamma(\alpha)} & x \geq 0 \\
     0 & \text{Otherwise}
  \end{cases}
\end{equation*}
Where we have
\begin{align*}
  \Gamma(\alpha) &= \int_{0}^{\infty}x^{\alpha -1}e^(-x) dx \\
                 &= (\alpha -1)!
\end{align*}
\subsection{Moment Generating Function $M(t)=E(e^{tX})$}

\begin{equation*}
    M(t)=\frac{\lambda^{\alpha}}{(\lambda -t)^{\alpha}}
\end{equation*}

\subsection{$\bm{E(X)}$}

\begin{equation*}
  E(X) = \frac{\alpha}{\lambda}
\end{equation*}

\subsection{$\bm{Var(X)}$}

\begin{equation*}
  Var(X)= \frac{\alpha}{\lambda^{2}}
\end{equation*}
\newpage
\section{Beta $X \sim B(\alpha,\beta)$}
\subsection{Probability Density Function $f(x)$}

\begin{equation*}
  f(x) =
  \begin{cases}
     \frac{x^{\alpha -1} (1-x)^{\beta -1}}{B(\alpha,\beta)} & x \in (0,1) \\
     0 & \text{Otherwise}
  \end{cases}
\end{equation*}
Where we have
\begin{align*}
  B(\alpha,\beta) &= \int_{0}^{1}x^{\alpha -1}(1-x)^{\beta -1} dx
\end{align*}

\subsection{$\bm{E(X)}$}

\begin{equation*}
  E(X) = \frac{\alpha}{\alpha + \beta}
\end{equation*}

\subsection{$\bm{Var(X)}$}

\begin{equation*}
  Var(X)= \frac{\alpha \beta}{(\alpha \beta)^{2} (\alpha + \beta + 1)}
\end{equation*}

\newpage
\section{Normal $X \sim N(\mu,\sigma^{2})$}
\subsection{Probability Density Function $f(x)$}

\begin{equation*}
  f(x) = \frac{1}{\sqrt{2\pi \sigma^{2}}}exp \left [- \frac{(x-\mu)^{2}}{2\sigma^{2}}\right]
\end{equation*}
Where we have $x \in \mathbb{R}$

\subsection{$\bm{E(X)}$}

\begin{equation*}
  E(X) = \mu
\end{equation*}

\subsection{$\bm{Var(X)}$}

\begin{equation*}
  Var(X)= \sigma^{2}
\end{equation*}

Also for normal distributions we can have that $X$ can become the standard normal distribution $Z \sim N(0,1)$ by
\begin{equation*}
  \frac{X-\mu}{\sigma^{2}}
\end{equation*}
\end{document}
